Classes/Monad/MonadExcept.v
@@ -7,11 +7,14 @@ Implicit Type A : Type.
 Class MonadExcept M {MM : Monad M} := {
   throw : ∀ {A}, M A;
   throw_left: ∀ {A B} (f : A → M B), throw >>= f = throw;
-  catch : ∀ {A} {JA : Joinable A A}, M A -> M A -> M A;
-  catch_left : ∀ {A} {JA : Joinable A A} (x : M A), catch throw x = x;
-  catch_right : ∀ {A} {JA : Joinable A A} (x : M A), catch x throw = x;
-  catch_return : ∀ {A} {JA : Joinable A A} (x : M A) (a : A),
-    catch (returnM a) x = returnM a;
+  catch : ∀ {A} {JA : Joinable A A} {JAI: JoinableIdem JA}, 
+    M A -> M A -> M A;
+  catch_left : ∀ {A} {JA : Joinable A A} {JAI : JoinableIdem JA} 
+    (x : M A), catch throw x = x;
+  catch_right : ∀ {A} {JA : Joinable A A} {JAI : JoinableIdem JA} 
+    (x : M A), catch x throw = x;
+  catch_return : ∀ {A} {JA : Joinable A A} {JAI : JoinableIdem JA} 
+    (x : M A) (a : A), catch (returnM a) x = returnM a;
 }.
 Arguments throw : simpl never.
 Arguments catch : simpl never.
