Classes/Monad/MonadJoin.v
@@ -2,15 +2,16 @@ Require Export Base.
 Require Import Classes.Monad Classes.Joinable Classes.Galois.
 
 Class MonadJoin M {MM : Monad M} : Type := {
-  mjoin : ∀ {A} {JA : Joinable A A}, M A → M A → M A;
-  mjoin_return : ∀ {A} {JA : Joinable A A} (x y : A),
+  mjoin : ∀ {A} {JA : Joinable A A} {JI : JoinableIdem JA}, M A → M A → M A;
+  mjoin_return : ∀ {A} {JA : Joinable A A} {JI : JoinableIdem JA} (x y : A),
     mjoin (returnM x) (returnM y) = returnM (x ⊔ y);
 }.
 Hint Rewrite @mjoin_return : monads.
 
 Infix "<⊔>" := mjoin (at level 40).
 
-Definition mjoin_option A {JA : Joinable A A} : option A → option A → option A :=
+Definition mjoin_option A {JA : Joinable A A} {JI : JoinableIdem JA} : 
+  option A → option A → option A :=
   λ m1 : option A, λ m2 : option A,
     match m1, m2 with
     | Some x, Some y => Some (x ⊔ y)
